fix lib_avl_mono/

lib_avl_mono/Impl.Trees.Types.fst
@@ -23,16 +23,16 @@ open Utils2
 // this is a compilation-time assert, see c/utils.c static_assert usage
 assume val avl_data_size_aux : v:U32.t{U32.v v <= 64}
 
-let avl_data_size : v:sc_union{U32.v avl_data_size_aux <= U32.v v} = Sc 64ul
+let avl_data_size : v:sc{U32.v avl_data_size_aux <= U32.v v} = 64ul
 
 open SizeClass
 open Main
 
 inline_for_extraction noextract
 val init_avl_scs (slab_region: array U8.t)
-  : Steel (size_class_struct)
+  : Steel (size_class_struct_sc)
   (A.varray slab_region)
-  (fun r -> size_class_vprop r)
+  (fun r -> size_class_vprop_sc r)
   (requires fun h0 ->
     A.is_full_array slab_region /\
     A.length slab_region = US.v metadata_max `FStar.Mul.op_Star` U32.v page_size /\
@@ -40,7 +40,7 @@ val init_avl_scs (slab_region: array U8.t)
     zf_u8 (A.asel slab_region h0)
   )
   (ensures fun _ r _ ->
-    r.size = avl_data_size /\
+    get_u32 r.size = avl_data_size /\
     r.slab_region == slab_region /\
     A.is_full_array r.slab_region
   )
@@ -61,13 +61,13 @@ noeq
 type mmap_md_slabs =
   {
     slab_region: array U8.t;
-    scs: v:size_class_struct{
-      v.size = avl_data_size /\
+    scs: v:size_class_struct_sc{
+      get_u32 v.size = avl_data_size /\
       v.slab_region == A.split_r slab_region 0sz /\
       A.is_full_array v.slab_region
     };
     lock : L.lock (
-      size_class_vprop scs `star`
+      size_class_vprop_sc scs `star`
       A.varray (A.split_l slab_region 0sz)
     );
   }
@@ -85,7 +85,7 @@ let init_mmap_md_slabs (_:unit)
     (A.ptr_of (A.split_r slab_region 0sz));
   assert (A.split_r slab_region 0sz == slab_region);
   let scs = init_avl_scs (A.split_r slab_region 0sz) in
-  let lock = L.new_lock (size_class_vprop scs `star` A.varray (A.split_l slab_region 0sz)) in
+  let lock = L.new_lock (size_class_vprop_sc scs `star` A.varray (A.split_l slab_region 0sz)) in
   return { slab_region; scs; lock; }
 #pop-options
 
@@ -179,7 +179,7 @@ let p : hpred data
       same_base_array ptr metadata_slabs.scs.slab_region /\
       UP.fits (A.offset (A.ptr_of ptr) - A.offset (A.ptr_of metadata_slabs.scs.slab_region)) /\
       A.offset (A.ptr_of ptr) - A.offset (A.ptr_of metadata_slabs.scs.slab_region) >= 0 /\
-      ((A.offset (A.ptr_of ptr) - A.offset (A.ptr_of metadata_slabs.scs.slab_region)) % U32.v page_size) % U32.v metadata_slabs.scs.size = 0)
+      ((A.offset (A.ptr_of ptr) - A.offset (A.ptr_of metadata_slabs.scs.slab_region)) % U32.v page_size) % U32.v (get_u32 metadata_slabs.scs.size) = 0)
     )
   )
 #pop-options
